some more work on random oracles in st2

examples/relational/ro.fst
@@ -21,7 +21,7 @@ type tag = b:bytes{length(b)=eta}
 
 (* TODO? *)
 (* an abstract relational predicate on correctly-generated entries *) 
-assume logic type safe (k:key) (k':key) (t:tag) (t':tag)  
+assume logic type safe (k:key) (t:tag) 
 
 
 type alloc = 
@@ -34,14 +34,61 @@ type state =
   { bad: bool; (* set iff any allocation has failed, e.g. bumped into the other's table *) 
     l:log }    (* the map ensures at most one entry per key *)
 
+
 type Ok : log -> log -> Type = 
   | Null: Ok [] [] 
-  | ConsH: k0:key -> k1:key-> t0:tag -> t1:tag { safe k0 k1 t0 t1 } 
-           -> log0:log -> log1:log { Ok log0 log1 } 
+  | ConsH: k0:key -> k1:key-> t0:tag{safe k0 t0} -> t1:tag{safe k1 t1} 
+           -> log0:log{is_None (assoc k0 log0)} 
+           -> log1:log{is_None (assoc k1 log1)} 
+           -> p: Ok log0 log1 
            -> Ok ((k0,(Hon,t0))::log0) ((k1,(Hon,t1))::log1)
   | ConsA: k:key -> t:tag 
-           -> log0:log -> log1:log { Ok log0 log1 } 
+           -> log0:log{is_None (assoc k log0)} 
+           -> log1:log{is_None (assoc k log1)} 
+           -> p: Ok log0 log1 
            -> Ok ((k ,(Adv,t ))::log0) ((k, (Adv,t ))::log1)
+
+val ok_adv_eq : l0:log -> l1:log -> p:Ok l0 l1 -> k:key 
+                -> Lemma 
+                   (requires True)
+                   (ensures (forall t. assoc k l0 = Some(Adv, t) <==> 
+                                       assoc k l1 = Some(Adv, t)))
+let rec ok_adv_eq l0 l1 p k = match p with
+        | Null -> ()
+        | ConsH _ _ _ _ tl0 tl1 p' -> ok_adv_eq tl0 tl1 p' k
+        | ConsA _ _ tl0 tl1 p' -> ok_adv_eq tl0 tl1 p' k
+
+(* Is there any way to show this using the previous lemma? *)
+val ok_adv_eq' : k:key 
+                -> Lemma 
+                   (requires True)
+                   (ensures (forall (l0:log) (l1:log).Ok l0 l1 ==> 
+                              (forall t. assoc k l0 = Some(Adv, t) <==> 
+                                         assoc k l1 = Some(Adv, t))))
+let ok_adv_eq' k = admit ()
+
+
+val ok_hon_safe : l0:log -> l1:log -> p:Ok l0 l1 -> k:key 
+                  -> Lemma 
+                     (requires True)
+                     (ensures (
+                                (forall t. assoc k l0 = Some(Hon, t) ==> safe k t)
+                                /\ (forall t. assoc k l1 = Some(Hon, t) ==> safe k t)))
+let rec ok_hon_safe l0 l1 p k = match p with
+        | Null -> ()
+        | ConsH _ _ _ _ tl0 tl1 p' -> ok_hon_safe tl0 tl1 p' k
+        | ConsA k' t' tl0 tl1 p' -> ok_hon_safe tl0 tl1 p' k
+
+(* Is there any way to show this using the previous lemma? *)
+val ok_hon_safe' : k:key 
+                -> Lemma 
+                   (requires True)
+                   (ensures (forall (l0:log) (l1:log).Ok l0 l1 ==> 
+                              (forall t. assoc k l0 = Some(Hon, t) ==> safe k t) 
+                              /\ (forall t. assoc k l1 = Some(Hon, t) ==> safe k t)))
+let ok_hon_safe' k = admit ()
+
+  
 
 type goodstate (s1:state) (s2:state) = 
             s1.bad = true \/ s2.bad = true \/ Ok s1.l s2.l
@@ -50,11 +97,11 @@ assume val s : ref state
 assume val sample_hon : k0:key -> k1:key -> 
                  ST2 (tag * tag)
                    (requires (fun _ -> True))
-                   (ensures (fun _ p _ -> safe k0 k1 (fst p) (snd p)))
+                   (ensures (fun h2' p h2 -> h2' = h2 /\ safe k0 (fst p) /\ safe k1 (snd p)))
 assume val sample_adv : unit -> 
                  ST2 (tag * tag)
                    (requires (fun _ -> True))
-                   (ensures (fun _ p _ -> fst p = snd p))
+                   (ensures (fun h2' p h2 -> h2' = h2 /\ fst p = snd p))
 
 val hash_hon:  k0:key -> k1:key ->
                ST2 (option tag * option tag)
@@ -62,7 +109,7 @@ val hash_hon:  k0:key -> k1:key ->
                (ensures (fun _ p h2 -> (sel (fst h2) s).bad \/ 
                                        (sel (snd h2) s).bad \/ 
                                        is_Some (fst p) /\ is_Some (snd p) /\ 
-                                          safe k0 k1 (Some.v(fst p)) (Some.v(snd p))))
+                                          safe k0 (Some.v(fst p)) /\ safe k1 (Some.v(snd p))))
 
 val hash_adv:  k:key -> 
                ST2 (option tag * option tag)
@@ -72,31 +119,34 @@ val hash_adv:  k:key ->
                                        is_Some (fst p) /\ is_Some (snd p) /\ 
                                           Some.v(fst p) = Some.v(snd p)))
                                       
-(* circumvent some typing problems... *)
+(* workaround for some typing problems... *)
 val add_some : tag -> Tot (option tag)
 let add_some t = Some t
 
-let hash_hon' k r =  match assoc k (!s).l with 
-  | Some (Hon,t) (* TODO ->  add_some t *) 
+let hash_hon' k r = match assoc k (!s).l with 
+  | Some (Hon,t) -> add_some t 
   | Some (Adv,t) -> s := {bad = true; l = (!s).l}; None
   | None         -> let t = r in 
                     s := {bad = (!s).bad; l= (k,(Hon,t))::(!s).l} ; 
                     add_some t 
 
-let hash_hon k0 k1  = let r0, r1 = sample_hon k0 k1 in 
+let hash_hon k0 k1  = ok_hon_safe' k0;
+                      ok_hon_safe' k1;
+                      let r0, r1 = sample_hon k0 k1 in 
                       (compose2 (fun k -> hash_hon' k r0) 
                                 (fun k -> hash_hon' k r1) 
                                 k0 k1)
 
 let hash_adv' k r =  match assoc k (!s).l with 
-  | Some (Adv,t) (* TODO -> add_some t *)
+  | Some (Adv,t) -> add_some t 
   | Some (Hon,t) -> s := {bad = true; l = (!s).l}; None
   | None         -> let t = r in 
                     s := {bad = (!s).bad; l= (k,(Adv,t))::(!s).l} ; 
                     add_some t 
 
-let hash_adv k  = let r0, r1 = sample_adv () in 
-                  (compose2 (fun k -> hash_adv' k r0) 
-                            (fun k -> hash_adv' k r1) 
-                            k k)
 
+let hash_adv k  = ok_adv_eq' k;
+                  let r0, r1 = sample_adv () in 
+                  compose2 (fun k -> hash_adv' k r0) 
+                           (fun k -> hash_adv' k r1) 
+                           k k
